library/data/monad/transformers.lean
@@ -1,0 +1,40 @@
+namespace monad
+
+class monad_transformer (transformer : ∀m [monad m], Type → Type) :=
+(is_monad : ∀m [monad m], monad (transformer m))
+(monad_lift : ∀m [monad m] A, m A → transformer m A)
+
+instance transformed_monad (m t) [monad_transformer t] [monad m] : monad (t m) :=
+monad_transformer.is_monad t m
+
+class has_monad_lift (m n : Type → Type) :=
+(monad_lift : ∀A, m A → n A)
+
+instance monad_transformer_lift (t m) [monad_transformer t] [monad m] : has_monad_lift m (t m) :=
+⟨monad_transformer.monad_lift t m⟩
+
+class has_monad_lift_t (m n : Type → Type) :=
+(monad_lift : ∀A, m A → n A)
+
+def monad_lift {m n} [has_monad_lift_t m n] {A} : m A → n A :=
+has_monad_lift_t.monad_lift n A
+
+prefix `♯ `:0 := monad_lift
+
+instance has_monad_lift_t_trans (m n o) [has_monad_lift n o] [has_monad_lift_t m n] : has_monad_lift_t m o :=
+⟨ λA (ma : m A), has_monad_lift.monad_lift o A $ has_monad_lift_t.monad_lift n A ma ⟩
+
+instance has_monad_lift_t_refl (m) [monad m] : has_monad_lift_t m m :=
+⟨ λA, id ⟩
+
+end monad
+
+namespace state_t
+
+def state_t_monad_lift (S) (m) [monad m] (A) (f : m A) : state_t S m A :=
+take state, do res ← f, return (res, state)
+
+instance (S) : monad.monad_transformer (state_t S) :=
+⟨ state_t.monad S, state_t_monad_lift S ⟩
+
+end state_t
