library/tools/super/cdcl.lean
@@ -1,0 +1,49 @@
+import .clause .clausifier .cdcl_solver
+open tactic expr monad super
+
+private meta def theory_solver_of_tactic (th_solver : tactic unit) : cdcl.solver (option cdcl.proof_term) :=
+do s ← state_t.read, ♯do
+hyps ← return $ s↣trail↣for (λe, e↣hyp),
+subgoal ← mk_meta_var s↣local_false,
+goals ← get_goals,
+set_goals [subgoal],
+hvs ← for hyps (λhyp, assertv hyp↣local_pp_name hyp↣local_type hyp),
+solved ← (do th_solver, now, return tt) <|> return ff,
+set_goals goals,
+if solved then do
+  proof ← instantiate_mvars subgoal,
+  proof' ← whnf proof, -- gets rid of the unnecessary asserts
+  return $ some proof'
+else
+  return none
+
+meta def cdcl_t (th_solver : tactic unit) : tactic unit := do
+as_refutation, local_false ← target,
+clauses ← clauses_of_context, clauses ← get_clauses_classical clauses,
+for clauses (λc, do c_pp ← pp c, clause.validate c <|> fail c_pp),
+res ← cdcl.solve (theory_solver_of_tactic th_solver) local_false clauses,
+match res with
+| (cdcl.result.unsat proof) := exact proof
+| (cdcl.result.sat interp) :=
+  let interp' := do e ← interp↣to_list, [if e↣2 = tt then e↣1 else not_ e↣1] in
+  do pp_interp ← pp interp',
+     fail (to_fmt "satisfying assignment: " ++ pp_interp)
+end
+
+meta def cdcl : tactic unit := cdcl_t skip
+
+example {a} : a → ¬a → false := by cdcl
+example {a} : a ∨ ¬a := by cdcl
+example {a b} : a → (a → b) → b := by cdcl
+example {a b c} : (a → b) → (¬a → b) → (b → c) → b ∧ c := by cdcl
+
+private meta def lit_unification : tactic unit :=
+do ls ← local_context, first $ do l ← ls, [do apply l, assumption]
+example {p : ℕ → Type _} : p 2 ∨ p 4 → (p (2*2) → p (2+0)) → p (1+1) :=
+by cdcl_t lit_unification
+
+example {p : ℕ → Prop} :
+        list.foldl (λf v, f ∧ (v ∨ ¬v)) true (map p (list.range 5)) :=
+begin (target >>= whnf >>= change), cdcl end
+
+example {a b c : Type _} : (a → b) → (b → c) → (a → c) := by cdcl
