library/tools/super/clause.lean
@@ -1,0 +1,250 @@
+import init.meta.tactic .utils .trim
+open expr list tactic monad decidable
+
+namespace super
+
+meta def is_local_not (local_false : expr) (e : expr) : option expr :=
+match e with
+| (pi _ _ a b) := if b = local_false then some a else none
+| _ := if local_false = false_ then is_not e else none
+end
+
+meta structure clause :=
+(num_quants : ℕ)
+(num_lits : ℕ)
+(proof : expr)
+(type : expr)
+(local_false : expr)
+
+namespace clause
+
+private meta def tactic_format (c : clause) : tactic format := do
+prf_fmt : format ← pp (proof c),
+type_fmt ← pp (type c),
+loc_fls_fmt ← pp c↣local_false,
+return $ prf_fmt ++ to_fmt " : " ++ type_fmt ++ to_fmt " (" ++
+  to_fmt (num_quants c) ++ to_fmt " quants, "
+  ++ to_fmt (num_lits c) ++ to_fmt " lits)"
+
+meta instance : has_to_tactic_format clause := ⟨tactic_format⟩
+
+meta def num_binders (c : clause) : ℕ := num_quants c + num_lits c
+
+meta def inst (c : clause) (e : expr) : clause :=
+(if num_quants c > 0
+  then mk (num_quants c - 1) (num_lits c)
+  else mk 0 (num_lits c - 1))
+(app (proof c) e) (instantiate_var (binding_body (type c)) e) c↣local_false
+
+meta def instn (c : clause) (es : list expr) : clause :=
+foldr (λe c', inst c' e) c es
+
+meta def open_const (c : clause) : tactic (clause × expr) := do
+n ← mk_fresh_name,
+b ← return $ local_const n (binding_name (type c)) (binding_info (type c)) (binding_domain (type c)),
+return (inst c b, b)
+
+meta def open_meta (c : clause) : tactic (clause × expr) := do
+b ← mk_meta_var (binding_domain (type c)),
+return (inst c b, b)
+
+meta def close_const (c : clause) (e : expr) : clause :=
+match e with
+| local_const uniq pp info t :=
+    let abst_type' := abstract_local (type c) (local_uniq_name e) in
+    let type' := pi pp binder_info.default t (abstract_local (type c) uniq) in
+    let abs_prf := abstract_local (proof c) uniq in
+    let proof' := lambdas [e] c↣proof in
+    if num_quants c > 0 ∨ has_var abst_type' then
+      { c with num_quants := c↣num_quants + 1, proof := proof', type := type' }
+    else
+      { c with num_lits := c↣num_lits + 1, proof := proof', type := type' }
+| _ := ⟨0, 0, default expr, default expr, default expr⟩
+end
+
+meta def open_constn : clause → ℕ → tactic (clause × list expr)
+| c 0 := return (c, nil)
+| c (n+1) := do
+  (c', b) ← open_const c,
+  (c'', bs) ← open_constn c' n,
+  return (c'', b::bs)
+
+meta def open_metan : clause → ℕ → tactic (clause × list expr)
+| c 0 := return (c, nil)
+| c (n+1) := do
+  (c', b) ← open_meta c,
+  (c'', bs) ← open_metan c' n,
+  return (c'', b::bs)
+
+meta def close_constn : clause → list expr → clause
+| c [] := c
+| c (b::bs') := close_const (close_constn c bs') b
+
+set_option eqn_compiler.max_steps 500
+
+private meta def parse_clause (local_false : expr) : expr → expr → tactic clause
+| proof (pi n bi d b) := do
+  lc_n ← mk_fresh_name,
+  lc ← return $ local_const lc_n n bi d,
+  c ← parse_clause (app proof lc) (instantiate_var b lc),
+  return $ c↣close_const $ local_const lc_n n binder_info.default d
+| proof (app (const ``not []) formula) := parse_clause proof (formula↣imp false_)
+| proof type :=
+if type = local_false then do
+  return { num_quants := 0, num_lits := 0, proof := proof, type := type, local_false := local_false }
+else do
+  univ ← infer_univ type,
+  not_type ← return $ imp type local_false,
+  parse_clause (lam `H binder_info.default not_type $ app (mk_var 0) proof) (imp not_type local_false)
+
+meta def of_proof_and_type (local_false proof type : expr) : tactic clause :=
+parse_clause local_false proof type
+
+meta def of_proof (local_false proof : expr) : tactic clause := do
+type ← infer_type proof,
+of_proof_and_type local_false proof type
+
+meta def of_classical_proof (proof : expr) : tactic clause :=
+of_proof false_ proof
+
+meta def inst_mvars (c : clause) : tactic clause := do
+proof' ← instantiate_mvars (proof c),
+type' ← instantiate_mvars (type c),
+return { c with proof := proof', type := type' }
+
+meta inductive literal
+| left : expr → literal
+| right : expr → literal
+
+namespace literal
+
+meta instance : decidable_eq literal := by mk_dec_eq_instance
+
+meta def formula : literal → expr
+| (left f) := f
+| (right f) := f
+
+meta def is_neg : literal → bool
+| (left _) := tt
+| (right _) := ff
+
+meta def is_pos (l : literal) : bool := bnot l↣is_neg
+
+meta def to_formula (l : literal) : tactic expr :=
+if is_neg l then mk_mapp ``not [some (formula l)]
+else return (formula l)
+
+meta def type_str : literal → string
+| (literal.left _) := "left"
+| (literal.right _) := "right"
+
+meta instance : has_to_tactic_format literal :=
+⟨λl, do
+pp_f ← pp l↣formula,
+return $ to_fmt l↣type_str ++ " (" ++ pp_f ++ ")"⟩
+
+end literal
+
+private meta def get_binding_body : expr → ℕ → expr
+| e 0 := e
+| e (i+1) := get_binding_body e↣binding_body i
+
+meta def get_binder (e : expr) (i : nat) :=
+binding_domain (get_binding_body e i)
+
+meta def validate (c : clause) : tactic unit := do
+concl ← return $ get_binding_body c↣type c↣num_binders,
+unify concl c↣local_false
+      <|> (do pp_concl ← pp concl, pp_lf ← pp c↣local_false,
+              fail $ to_fmt "wrong local false: " ++ pp_concl ++ " =!= " ++ pp_lf),
+type' ← infer_type c↣proof,
+unify c↣type type' <|> (do pp_ty ← pp c↣type, pp_ty' ← pp type',
+                           fail (to_fmt "wrong type: " ++ pp_ty ++ " =!= " ++ pp_ty'))
+
+meta def get_lit (c : clause) (i : nat) : literal :=
+let bind := get_binder (type c) (num_quants c + i) in
+match is_local_not c↣local_false bind with
+| some formula := literal.right formula
+| none         := literal.left bind
+end
+
+meta def lits_where (c : clause) (p : literal → bool) : list nat :=
+list.filter (λl, p (get_lit c l)) (range (num_lits c))
+
+meta def get_lits (c : clause) : list literal :=
+list.map (get_lit c) (range c↣num_lits)
+
+meta def is_maximal (gt : expr → expr → bool) (c : clause) (i : nat) : bool :=
+list.empty (list.filter (λj, gt (get_lit c j)↣formula (get_lit c i)↣formula) (range c↣num_lits))
+
+meta def normalize (c : clause) : tactic clause := do
+opened  ← open_constn c (num_binders c),
+lconsts_in_types ← return $ contained_lconsts_list (list.map local_type opened.2),
+quants' ← return $ list.filter (λlc, rb_map.contains lconsts_in_types (local_uniq_name lc))
+                                                      opened.2,
+lits' ← return $ list.filter (λlc, ¬rb_map.contains lconsts_in_types (local_uniq_name lc))
+                                                     opened.2,
+return $ close_constn opened.1 (quants' ++ lits')
+
+meta def whnf_head_lit (c : clause) : tactic clause := do
+atom' ← whnf $ literal.formula $ get_lit c 0,
+return $
+if literal.is_neg (get_lit c 0) then
+  { c with type := imp atom' (binding_body c↣type) }
+else
+  { c with type := imp (app (const ``not []) atom') c↣type↣binding_body }
+
+end clause
+
+meta def unify_lit (l1 l2 : clause.literal) : tactic unit :=
+if clause.literal.is_pos l1 = clause.literal.is_pos l2 then
+  unify_core transparency.none (clause.literal.formula l1) (clause.literal.formula l2)
+else
+  fail "cannot unify literals"
+
+-- FIXME: this is most definitely broken with meta-variables that were already in the goal
+meta def sort_and_constify_metas : list expr → tactic (list expr)
+| exprs_with_metas := do
+inst_exprs ← mapm instantiate_mvars exprs_with_metas,
+metas ← return $ inst_exprs >>= get_metas,
+match list.filter (λm, ¬has_meta_var (get_meta_type m)) metas with
+| [] :=
+     if metas^.empty then
+       return []
+     else do
+       for' metas (λm, do trace (expr.to_string m), t ← infer_type m, trace (expr.to_string t)),
+       fail "could not sort metas"
+| ((mvar n t) :: _) := do
+  t' ← infer_type (mvar n t),
+  uniq ← mk_fresh_name,
+  c ← return (local_const uniq uniq binder_info.default t'),
+  unify c (mvar n t),
+  rest ← sort_and_constify_metas metas,
+  return (rest ++ [c])
+| _ := failed
+end
+
+namespace clause
+
+meta def meta_closure (metas : list expr) (qf : clause) : tactic clause := do
+bs ← sort_and_constify_metas metas,
+qf' ← clause.inst_mvars qf,
+clause.inst_mvars $ clause.close_constn qf' bs
+
+private meta def distinct' (local_false : expr) : list expr → expr → clause
+| [] proof := ⟨ 0, 0, proof, local_false, local_false ⟩
+| (h::hs) proof :=
+  let (dups, rest) := partition (λh' : expr, h↣local_type = h'↣local_type) hs,
+      proof_wo_dups := foldl (λproof (h' : expr),
+                              instantiate_var (abstract_local proof h'↣local_uniq_name) h)
+                         proof dups in
+    (distinct' rest proof_wo_dups)↣close_const h
+
+meta def distinct (c : clause) : tactic clause := do
+(qf, vs) ← c↣open_constn c↣num_quants,
+(fls, hs) ← qf↣open_constn qf↣num_lits,
+return $ (distinct' c↣local_false hs fls↣proof)↣close_constn vs
+
+end clause
+
+end super
