library/tools/super/datatypes.lean
@@ -1,0 +1,52 @@
+import .clause_ops .prover_state data.monad.transformers
+open expr tactic monad
+
+namespace super
+
+meta def has_diff_constr_eq_l (c : clause) : tactic bool := do
+env ← get_env,
+return $ list.bor $ do
+  l ← c↣get_lits,
+  guard l↣is_neg,
+  return $ match is_eq l↣formula with
+  | some (lhs, rhs) :=
+    if env↣is_constructor_app lhs ∧ env↣is_constructor_app rhs ∧
+       lhs↣get_app_fn↣const_name ≠ rhs↣get_app_fn↣const_name then
+      tt
+    else
+      ff
+  | _ := ff
+  end
+
+meta def diff_constr_eq_l_pre := preprocessing_rule $
+filter (λc, lift bnot $♯ has_diff_constr_eq_l c↣c)
+
+meta def try_no_confusion_eq_r (c : clause) (i : ℕ) : tactic (list clause) :=
+on_right_at' c i $ λhyp,
+  match is_eq hyp↣local_type with
+  | some (lhs, rhs) := do
+    env ← get_env,
+    lhs ← whnf lhs, rhs ← whnf rhs,
+    guard $ env↣is_constructor_app lhs ∧ env↣is_constructor_app rhs,
+    pr ← mk_app (lhs↣get_app_fn↣const_name↣get_prefix <.> "no_confusion") [false_, lhs, rhs, hyp],
+    -- FIXME: change to local false ^^
+    ty ← infer_type pr, ty ← whnf ty,
+    pr ← to_expr `(@eq.mpr _ %%ty rfl %%pr), -- FIXME
+    return [([], pr)]
+  | _ := failed
+  end
+
+example (x y : ℕ) (h : nat.zero = nat.succ nat.zero) (h2 : nat.succ x = nat.succ y) : true := by do
+h ← get_local `h >>= clause.of_classical_proof,
+h2 ← get_local `h2 >>= clause.of_classical_proof,
+cs ← try_no_confusion_eq_r h 0,
+for' cs clause.validate,
+cs ← try_no_confusion_eq_r h2 0,
+for' cs clause.validate,
+to_expr `(trivial) >>= exact
+
+@[super.inf]
+meta def datatype_infs : inf_decl := inf_decl.mk 10 $ take given, do
+sequence' (do i ← list.range given↣c↣num_lits, [inf_if_successful 0 given $ try_no_confusion_eq_r given↣c i])
+
+end super
