library/tools/super/defs.lean
@@ -1,0 +1,31 @@
+import .clause_ops .prover_state
+open tactic expr monad
+
+namespace super
+
+-- FIXME: how to cleanly unfold one level of definitions?
+-- what should one level even be? consider dvd->has_dvd->nat_has_dvd->...
+meta def try_unfold_one_def (type : expr) : tactic expr := do
+whnf type
+
+meta def try_unfold_def_left (c : clause) (i : ℕ) : tactic (list clause) :=
+on_left_at c i $ λt, do
+  t' ← try_unfold_one_def t,
+  ht' ← mk_local_def `h t',
+  return [([ht'], ht')]
+
+meta def try_unfold_def_right (c : clause) (i : ℕ) : tactic (list clause) :=
+on_right_at c i $ λh, do
+  t' ← try_unfold_one_def h↣local_type,
+  hnt' ← mk_local_def `h (imp t' c↣local_false),
+  return [([hnt'], app hnt' h)]
+
+@[super.inf]
+meta def unfold_def_inf : inf_decl := inf_decl.mk 40 $ take given, sequence' $ do
+r ← [try_unfold_def_right, try_unfold_def_left],
+-- NOTE: we cannot restrict to selected literals here
+-- as this might prevent factoring, e.g. _n>0_ ∨ is_pos(0)
+i ← list.range given↣c↣num_lits,
+[inf_if_successful 3 given (r given↣c i)]
+
+end super
