library/tools/super/examples.lean
@@ -1,0 +1,83 @@
+import .prover
+open tactic
+
+constant nat_has_dvd : has_dvd nat
+attribute [instance] nat_has_dvd
+
+noncomputable def prime (n : ℕ) := ∀d, dvd d n → d = 1 ∨ d = n
+axiom dvd_refl (m : ℕ) : dvd m m
+axiom dvd_mul (m n k : ℕ) : dvd m n → dvd m (n*k)
+
+axiom nat_mul_cancel_one (m n : ℕ) : m = m * n → n = 1
+
+example {m n : ℕ} : prime (m * n) → m = 1 ∨ n = 1 :=
+begin with_lemmas dvd_refl dvd_mul nat_mul_cancel_one, super end
+
+example : nat.zero ≠ nat.succ nat.zero := by super
+example (x y : ℕ) : nat.succ x = nat.succ y → x = y := by super
+example (i) (a b c : i) : [a,b,c] = [b,c,a] -> a = b ∧ b = c := by super
+
+definition is_positive (n : ℕ) := n > 0
+example (n : ℕ) : n > 0 ↔ is_positive n := by super
+
+example (m n : ℕ) : 0 + m = 0 + n → m = n :=
+by super with nat.zero_add
+
+local attribute [simp] nat.zero_add nat.succ_add
+@[simp] lemma nat_add_succ (m n : ℕ) : m + nat.succ n = nat.succ (m + n) := rfl
+@[simp] lemma nat_zero_has_zero : nat.zero = 0 := rfl
+example : ∀x y : ℕ, x + y = y + x :=
+begin intros, induction x, super, super end
+
+example (i) [inhabited i] : nonempty i := by super
+example (i) [nonempty i] : ¬(inhabited i → false) := by super
+
+example : nonempty ℕ := by super
+example : ¬(inhabited ℕ → false) := by super
+
+example {a b} : ¬(b ∨ ¬a) ∨ (a → b) := by super
+example {a} : a ∨ ¬a := by super
+example {a} : (a ∧ a) ∨ (¬a ∧ ¬a) := by super
+example (i) (c : i) (p : i → Prop) (f : i → i) :
+  p c → (∀x, p x → p (f x)) → p (f (f (f c))) := by super
+
+example (i) (p : i → Prop) : ∀x, p x → ∃x, p x := by super
+
+example (i) [nonempty i] (p : i → i → Prop) : (∀x y, p x y) → ∃x, ∀z, p x z := by super
+
+example (i) [nonempty i] (p : i → Prop) : (∀x, p x) → ¬¬∀x, p x := by super
+
+-- Requires non-empty domain.
+example {i} [nonempty i] (p : i → Prop) :
+  (∀x y, p x ∨ p y) → ∃x y, p x ∧ p y := by super
+
+example (i) (a b : i) (p : i → Prop) (H : a = b) : p b → p a :=
+by super
+
+example (i) (a b : i) (p : i → Prop) (H : a = b) : p a → p b :=
+by super
+
+example (i) (a b : i) (p : i → Prop) (H : a = b) : p b = p a :=
+by super
+
+example (i) (c : i) (p : i → Prop) (f g : i → i) :
+p c → (∀x, p x → p (f x)) → (∀x, p x → f x = g x) → f (f c) = g (g c) :=
+by super
+
+example (i) (p q : i → i → Prop) (a b c d : i) :
+  (∀x y z, p x y ∧ p y z → p x z) →
+  (∀x y z, q x y ∧ q y z → q x z) →
+  (∀x y, q x y → q y x) →
+  (∀x y, p x y ∨ q x y) →
+  p a b ∨ q c d :=
+by super
+
+-- This example from Davis-Putnam actually requires a non-empty domain
+example (i) [nonempty i] (f g : i → i → Prop) :
+  ∃x y, ∀z, (f x y → f y z ∧ f z z) ∧ (f x y ∧ g x y → g x z ∧ g z z) :=
+by super
+
+example (person) [nonempty person] (drinks : person → Prop) :
+  ∃canary, drinks canary → ∀other, drinks other := by super
+
+example {p q : ℕ → Prop} {r} : (∀x y, p x ∧ q y ∧ r) -> ∀x, (p x ∧ r ∧ q x) := by super
