library/tools/super/factoring.lean
@@ -1,0 +1,46 @@
+import .clause .prover_state .subsumption
+open tactic expr monad
+
+namespace super
+
+variable gt : expr → expr → bool
+
+meta def inst_lit (c : clause) (i : nat) (e : expr) : tactic clause := do
+opened ← clause.open_constn c i,
+return $ clause.close_constn (clause.inst opened.1 e) opened.2
+
+private meta def try_factor' (c : clause) (i j : nat) : tactic clause := do
+qf ← clause.open_metan c c↣num_quants,
+unify_lit (qf↣1↣get_lit i) (qf↣1↣get_lit j),
+qfi ← clause.inst_mvars qf.1,
+guard $ clause.is_maximal gt qfi i,
+at_j ← clause.open_constn qf.1 j,
+hyp_i ← option.to_monad (list.nth at_j.2 i),
+clause.meta_closure qf↣2 $ (at_j↣1↣inst hyp_i)↣close_constn at_j↣2
+
+meta def try_factor (c : clause) (i j : nat) : tactic clause :=
+if i > j then try_factor' gt c j i else try_factor' gt c i j
+
+meta def try_infer_factor (c : derived_clause) (i j : nat) : prover unit := do
+f ← ♯ try_factor gt c↣c i j,
+ss ← ♯ does_subsume f c↣c,
+if ss then do
+  f ← mk_derived f c↣sc↣sched_now,
+  add_inferred f,
+  remove_redundant c↣id [f]
+else do
+  inf_score 1 [c↣sc] >>= mk_derived f >>= add_inferred
+
+@[super.inf]
+meta def factor_inf : inf_decl := inf_decl.mk 40 $
+take given, do gt ← get_term_order, sequence' $ do
+  i ← given↣selected,
+  j ← list.range given↣c↣num_lits,
+  return $ try_infer_factor gt given i j <|> return ()
+
+meta def factor_dup_lits_pre := preprocessing_rule $ take new, do
+♯ for new $ λdc, do
+  dist ← dc↣c↣distinct,
+  return { dc with c := dist }
+
+end super
