library/tools/super/inhabited.lean
@@ -1,0 +1,65 @@
+import .clause_ops .prover_state
+open expr tactic monad
+
+namespace super
+
+meta def try_nonempty_lookup_left (c : clause) : tactic (list clause) :=
+on_first_left_dn c $ λhnx,
+  match is_local_not c↣local_false hnx↣local_type with
+  | some type := do
+    univ ← infer_univ type,
+    lf_univ ← infer_univ c↣local_false,
+    guard $ lf_univ = level.zero,
+    inst ← mk_instance (app (const ``nonempty [univ]) type),
+    instt ← infer_type inst,
+    return [([], app_of_list (const ``nonempty.elim [univ])
+                             [type, c↣local_false, inst, hnx])]
+  | _ := failed
+  end
+
+meta def try_nonempty_left (c : clause) : tactic (list clause) :=
+on_first_left c $ λprop,
+  match prop with
+  | (app (const ``nonempty [u]) type) := do
+    x ← mk_local_def `x type,
+    return [([x], app_of_list (const ``nonempty.intro [u]) [type, x])]
+  | _ := failed
+  end
+
+meta def try_nonempty_right (c : clause) : tactic (list clause) :=
+on_first_right c $ λhnonempty,
+  match hnonempty↣local_type with
+  | (app (const ``nonempty [u]) type) := do
+    lf_univ ← infer_univ c↣local_false,
+    guard $ lf_univ = level.zero,
+    hnx ← mk_local_def `nx (imp type c↣local_false),
+    return [([hnx], app_of_list (const ``nonempty.elim [u])
+                                [type, c↣local_false, hnonempty, hnx])]
+  | _ := failed
+  end
+
+meta def try_inhabited_left (c : clause) : tactic (list clause) :=
+on_first_left c $ λprop,
+  match prop with
+  | (app (const ``inhabited [u]) type) := do
+    x ← mk_local_def `x type,
+    return [([x], app_of_list (const ``inhabited.mk [u]) [type, x])]
+  | _ := failed
+  end
+
+meta def try_inhabited_right (c : clause) : tactic (list clause) :=
+on_first_right' c $ λhinh,
+  match hinh↣local_type with
+  | (app (const ``inhabited [u]) type) :=
+    return [([], app_of_list (const ``inhabited.default [u]) [type, hinh])]
+  | _ := failed
+  end
+
+@[super.inf]
+meta def inhabited_infs : inf_decl := inf_decl.mk 10 $ take given, do
+for' [try_nonempty_lookup_left,
+       try_nonempty_left, try_nonempty_right,
+       try_inhabited_left, try_inhabited_right] $ λr,
+      simp_if_successful given (r given↣c)
+
+end super
