library/tools/super/lpo.lean
@@ -1,0 +1,66 @@
+-- Polytime version of lexicographic path order as described in:
+-- Things to know when implementing LPO, Bernd Löchner, ESFOR 2004
+import .utils
+open expr decidable monad
+
+def lex {T} [decidable_eq T] (gt : T → T → bool) : list T → list T → bool
+| (s::ss) (t::ts) := if s = t then lex ss ts else gt s t
+| _ _ := ff
+
+def majo {T} (gt : T → T → bool) (s : T) : list T → bool
+| [] := tt
+| (t::ts) := gt s t && majo ts
+
+meta def alpha (lpo : expr → expr → bool) : list expr → expr → bool
+| [] _ := ff
+| (s::ss) t := to_bool (s = t) || lpo s t || alpha ss t
+
+meta def lex_ma (lpo : expr → expr → bool) (s t : expr) : list expr → list expr → bool
+| (si::ss) (ti::ts) :=
+  if si = ti then lex_ma ss ts
+  else if lpo si ti then majo lpo s ts
+  else alpha lpo (si::ss) t
+| _ _ := ff
+
+meta def lpo (prec_gt : expr → expr → bool) : expr → expr → bool | s t :=
+if prec_gt (get_app_fn s) (get_app_fn t) then majo lpo s (get_app_args t)
+else if get_app_fn s = get_app_fn t then lex_ma lpo s t (get_app_args s) (get_app_args t)
+else alpha lpo (get_app_args s) t
+
+meta def prec_gt_of_name_list (ns : list name) : expr → expr → bool :=
+let nis := rb_map.of_list (list.zip_with_index ns) in
+λs t, match (rb_map.find nis (name_of_funsym s), rb_map.find nis (name_of_funsym t)) with
+| (some si, some ti) := to_bool (si > ti)
+| _ := ff
+end
+
+open tactic
+example (m n : ℕ) : true := by do
+e₁ ← to_expr `((0 + (m : ℕ)) + 0),
+e₂ ← to_expr `(0 + (0 + (m : ℕ))),
+e₃ ← to_expr `(0 + (m : ℕ)),
+prec ← return (contained_funsyms e₁)↣keys,
+prec_gt ← return $ prec_gt_of_name_list prec,
+guard $ lpo prec_gt e₁ e₃,
+guard $ lpo prec_gt e₂ e₃,
+to_expr `(trivial) >>= apply
+
+/-
+open tactic
+example (i : Type) (f : i → i) (c d x : i) : true := by do
+ef ← get_local `f, ec ← get_local `c, ed ← get_local `d,
+syms ← return [ef,ec,ed],
+prec_gt ← return $ prec_gt_of_name_list (list.map local_uniq_name [ef, ec, ed]),
+sequence' (do s1 ← syms, s2 ← syms, return (do
+  s1_fmt ← pp s1, s2_fmt ← pp s2,
+  trace (s1_fmt ++ to_fmt " > " ++ s2_fmt ++ to_fmt ": " ++ to_fmt (prec_gt s1 s2))
+)),
+
+exprs ← @mapM tactic _ _ _ to_expr [`(f c), `(f (f c)), `(f d), `(f x), `(f (f x))],
+sequence' (do e1 ← exprs, e2 ← exprs, return (do
+  e1_fmt ← pp e1, e2_fmt ← pp e2,
+  trace (e1_fmt ++ to_fmt" > " ++ e2_fmt ++ to_fmt": " ++ to_fmt (lpo prec_gt e1 e2))
+)),
+
+mk_const ``true.intro >>= apply
+-/
