library/tools/super/misc_preprocessing.lean
@@ -1,0 +1,33 @@
+import .clause .prover_state
+open expr list monad
+
+namespace super
+
+meta def is_taut (c : clause) : tactic bool := do
+qf ← c^.open_constn c↣num_quants,
+return $ list.bor $ do
+  l1 ← qf^.1^.get_lits, guard l1^.is_neg,
+  l2 ← qf^.1^.get_lits, guard l2^.is_pos,
+  [decidable.to_bool $ l1^.formula = l2^.formula]
+
+open tactic
+example (i : Type) (p : i → i → Type) (c : i) (h : ∀ (x : i), p x c → p x c) : true := by do
+h ← get_local `h, hcls ← clause.of_classical_proof h,
+taut ← is_taut hcls,
+when (¬taut) failed,
+to_expr `(trivial) >>= apply
+
+meta def tautology_removal_pre : prover unit :=
+preprocessing_rule $ λnew, filter (λc, lift bnot $♯ is_taut c↣c) new
+
+meta def remove_duplicates : list derived_clause → list derived_clause
+| [] := []
+| (c :: cs) :=
+  let (same_type, other_type) := partition (λc' : derived_clause, c'↣c↣type = c↣c↣type) cs in
+  { c with sc := foldl score.min c↣sc (same_type↣for $ λc, c↣sc) } :: remove_duplicates other_type
+
+meta def remove_duplicates_pre : prover unit :=
+preprocessing_rule $ λnew,
+return $ remove_duplicates new
+
+end super
