library/tools/super/prover_state.lean
@@ -1,0 +1,433 @@
+import .clause .lpo .cdcl_solver data.monad.transformers
+open tactic monad expr
+
+namespace super
+
+structure score :=
+(priority : ℕ)
+(in_sos : bool)
+(cost : ℕ)
+(age : ℕ)
+
+namespace score
+def prio.immediate : ℕ := 0
+def prio.default   : ℕ := 1
+def prio.never     : ℕ := 2
+
+def sched_default (sc : score) : score := { sc with priority := prio.default }
+def sched_now (sc : score) : score := { sc with priority := prio.immediate }
+
+def inc_cost (sc : score) (n : ℕ) : score := { sc with cost := sc↣cost + n }
+
+def min (a b : score) : score :=
+{ priority := nat.min a↣priority b↣priority,
+  in_sos := a↣in_sos && b↣in_sos,
+  cost := nat.min a↣cost b↣cost,
+  age := nat.min a↣age b↣age }
+
+def combine (a b : score) : score :=
+{ priority := nat.max a↣priority b↣priority,
+  in_sos := a↣in_sos && b↣in_sos,
+  cost := a↣cost + b↣cost,
+  age := nat.max a↣age b↣age }
+end score
+
+namespace score
+meta instance : has_to_string score :=
+⟨λe, "[" ++ to_string e↣priority ++
+     "," ++ to_string e↣cost ++
+     "," ++ to_string e↣age ++
+     ",sos=" ++ to_string e↣in_sos ++ "]"⟩
+end score
+
+def clause_id := ℕ
+namespace clause_id
+def to_nat (id : clause_id) : ℕ := id
+instance : decidable_eq clause_id := nat.decidable_eq
+instance : has_ordering clause_id := nat.has_ordering
+end clause_id
+
+meta structure derived_clause :=
+(id : clause_id)
+(c : clause)
+(selected : list ℕ)
+(assertions : list expr)
+(sc : score)
+
+namespace derived_clause
+
+meta instance : has_to_tactic_format derived_clause :=
+⟨λc, do
+c_fmt ← pp c↣c,
+ass_fmt ← pp (c↣assertions↣for (λa, a↣local_type)),
+return $
+to_string c↣sc ++ " " ++
+c_fmt ++ " <- " ++ ass_fmt ++
+" (selected: " ++ to_fmt c↣selected ++
+")"
+⟩
+
+meta def clause_with_assertions (ac : derived_clause) : clause :=
+ac↣c↣close_constn ac↣assertions
+
+end derived_clause
+
+meta structure locked_clause :=
+(dc : derived_clause)
+(reasons : list (list expr))
+
+namespace locked_clause
+
+meta instance : has_to_tactic_format locked_clause :=
+⟨λc, do
+c_fmt ← pp c↣dc,
+reasons_fmt ← pp (c↣reasons↣for (λr, r↣for (λa, a↣local_type))),
+return $ c_fmt ++ " (locked in case of: " ++ reasons_fmt ++ ")"
+⟩
+
+end locked_clause
+
+meta structure prover_state :=
+(active : rb_map clause_id derived_clause)
+(passive : rb_map clause_id derived_clause)
+(newly_derived : list derived_clause)
+(prec : list expr)
+(locked : list locked_clause)
+(local_false : expr)
+(sat_solver : cdcl.state)
+(current_model : rb_map expr bool)
+(sat_hyps : rb_map expr (expr × expr))
+(needs_sat_run : bool)
+(clause_counter : nat)
+
+open prover_state
+
+private meta def join_with_nl : list format → format :=
+list.foldl (λx y, x ++ format.line ++ y) format.nil
+
+private meta def prover_state_tactic_fmt (s : prover_state) : tactic format := do
+active_fmts ← mapm pp $ rb_map.values s↣active,
+passive_fmts ← mapm pp $ rb_map.values s↣passive,
+new_fmts ← mapm pp s↣newly_derived,
+locked_fmts ← mapm pp s↣locked,
+sat_fmts ← mapm pp s↣sat_solver↣clauses,
+prec_fmts ← mapm pp s↣prec,
+return (join_with_nl
+  ([to_fmt "active:"] ++ map (append (to_fmt "  ")) active_fmts ++
+  [to_fmt "passive:"] ++ map (append (to_fmt "  ")) passive_fmts ++
+  [to_fmt "new:"] ++ map (append (to_fmt "  ")) new_fmts ++
+  [to_fmt "locked:"] ++ map (append (to_fmt "  ")) locked_fmts ++
+  [to_fmt "sat formulas:"] ++ map (append (to_fmt "  ")) sat_fmts ++
+  [to_fmt "precedence order: " ++ to_fmt prec_fmts]))
+
+meta instance : has_to_tactic_format prover_state :=
+⟨prover_state_tactic_fmt⟩
+
+meta def prover := state_t prover_state tactic
+meta instance : monad prover := state_t.monad _ _
+meta instance : has_monad_lift tactic prover := monad.monad_transformer_lift (state_t prover_state) tactic
+
+meta def prover.fail {A B : Type} [has_to_format B] (msg : B) : prover A := ♯ @tactic.fail A _ _ msg
+
+meta def prover.failed {A : Type} : prover A :=
+prover.fail "failed"
+
+meta def prover.orelse {A : Type} (p1 p2 : prover A) : prover A :=
+take state, p1 state <|> p2 state
+
+meta instance : alternative prover :=
+alternative.mk (@monad.map _ _)
+  (@applicative.pure _ (monad_is_applicative prover))
+  (@applicative.seq _ (monad_is_applicative prover))
+  @prover.failed
+  @prover.orelse
+
+meta def selection_strategy := derived_clause → prover derived_clause
+
+meta def get_active : prover (rb_map clause_id derived_clause) :=
+do state ← state_t.read, return state↣active
+
+meta def add_active (a : derived_clause) : prover unit :=
+do state ← state_t.read,
+state_t.write { state with active := state↣active↣insert a↣id a }
+
+meta def get_passive : prover (rb_map clause_id derived_clause) :=
+lift passive state_t.read
+
+meta def get_precedence : prover (list expr) :=
+do state ← state_t.read, return state↣prec
+
+meta def get_term_order : prover (expr → expr → bool) := do
+state ← state_t.read,
+return $ lpo (prec_gt_of_name_list (map name_of_funsym state↣prec))
+
+private meta def set_precedence (new_prec : list expr) : prover unit :=
+do state ← state_t.read, state_t.write { state with prec := new_prec }
+
+meta def register_consts_in_precedence (consts : list expr) := do
+p ← get_precedence,
+p_set ← return (rb_map.set_of_list (map name_of_funsym p)),
+new_syms ← return $ list.filter (λc, ¬p_set↣contains (name_of_funsym c)) consts,
+set_precedence (new_syms ++ p)
+
+meta def in_sat_solver {A} (cmd : cdcl.solver A) : prover A := do
+state ← state_t.read,
+result ← ♯ cmd state↣sat_solver,
+state_t.write { state with sat_solver := result↣2 },
+return result↣1
+
+meta def collect_ass_hyps (c : clause) : prover (list expr) :=
+let lcs := contained_lconsts c↣proof in
+do st ← state_t.read,
+return (do
+  hs ← st↣sat_hyps↣values,
+  h ← [hs↣1, hs↣2],
+  guard $ lcs↣contains h↣local_uniq_name,
+  [h])
+
+meta def get_clause_count : prover ℕ :=
+do s ← state_t.read, return s↣clause_counter
+
+meta def get_new_cls_id : prover clause_id := do
+state ← state_t.read,
+state_t.write { state with clause_counter := state↣clause_counter + 1 },
+return state↣clause_counter
+
+meta def mk_derived (c : clause) (sc : score) : prover derived_clause := do
+ass ← collect_ass_hyps c,
+id ← ♯ get_new_cls_id,
+return { id := id, c := c, selected := [], assertions := ass, sc := sc }
+
+meta def add_inferred (c : derived_clause) : prover unit := do
+c' ← ♯c↣c↣normalize, c' ← return { c with c := c' },
+register_consts_in_precedence (contained_funsyms c'↣c↣type)↣values,
+state ← state_t.read,
+state_t.write { state with newly_derived := c' :: state↣newly_derived }
+
+
+
+-- FIXME: what if we've seen the variable before, but with a weaker score?
+meta def mk_sat_var (v : expr) (suggested_ph : bool) (suggested_ev : score) : prover unit :=
+do st ← state_t.read, if st↣sat_hyps↣contains v then return () else do
+hpv ← ♯ mk_local_def `h v,
+hnv ← ♯ mk_local_def `hn $ imp v st↣local_false,
+state_t.modify $ λst, { st with sat_hyps := st↣sat_hyps↣insert v (hpv, hnv) },
+in_sat_solver $ cdcl.mk_var_core v suggested_ph,
+match v with
+| (pi _ _ _ _) := do
+  c ← ♯ clause.of_proof st↣local_false hpv,
+  mk_derived c suggested_ev >>= add_inferred
+| _ := do cp ← ♯ clause.of_proof st↣local_false hpv, mk_derived cp suggested_ev >>= add_inferred,
+          cn ← ♯ clause.of_proof st↣local_false hnv, mk_derived cn suggested_ev >>= add_inferred
+end
+
+meta def get_sat_hyp_core (v : expr) (ph : bool) : prover (option expr) :=
+flip monad.lift state_t.read $ λst,
+  match st↣sat_hyps↣find v with
+  | some (hp, hn) := some $ if ph then hp else hn
+  | none := none
+  end
+
+meta def get_sat_hyp (v : expr) (ph : bool) : prover expr :=
+do hyp_opt ← get_sat_hyp_core v ph,
+match hyp_opt with
+| some hyp := return hyp
+| none := prover.fail $ "unknown sat variable: " ++ v↣to_string
+end
+
+meta def add_sat_clause (c : clause) (suggested_ev : score) : prover unit := do
+c ← ♯ c↣distinct,
+already_added ← flip monad.lift state_t.read $ λst, decidable.to_bool $
+                     c↣type ∈ st↣sat_solver↣clauses↣for (λd, d↣type),
+if already_added then return () else do
+for c↣get_lits $ λl, mk_sat_var l↣formula l↣is_neg suggested_ev,
+in_sat_solver $ cdcl.mk_clause c,
+state_t.modify $ λst, { st with needs_sat_run := tt }
+
+meta def sat_eval_lit (v : expr) (pol : bool) : prover bool :=
+do v_st ← flip monad.lift state_t.read $ λst, st↣current_model↣find v,
+match v_st with
+| some ph := return $ if pol then ph else bnot ph
+| none := return tt
+end
+
+meta def sat_eval_assertion (assertion : expr) : prover bool :=
+do lf ← flip monad.lift state_t.read $ λst, st↣local_false,
+match is_local_not lf assertion↣local_type with
+| some v := sat_eval_lit v ff
+| none := sat_eval_lit assertion↣local_type tt
+end
+
+meta def sat_eval_assertions : list expr → prover bool
+| (a::ass) := do v_a ← sat_eval_assertion a,
+if v_a then
+sat_eval_assertions ass
+else
+return ff
+| [] := return tt
+
+private meta def intern_clause (c : derived_clause) : prover derived_clause := do
+hyp_name ← ♯ get_unused_name (mk_simple_name $ "clause_" ++ to_string c↣id↣to_nat) none,
+c' ← return $ c↣c↣close_constn c↣assertions,
+♯ assertv hyp_name c'↣type c'↣proof,
+proof' ← ♯ get_local hyp_name,
+type ← ♯ infer_type proof', -- FIXME: otherwise ""
+return { c with c := { (c↣c : clause) with proof := app_of_list proof' c↣assertions } }
+
+meta def register_as_passive (c : derived_clause) : prover unit := do
+c ← intern_clause c,
+ass_v ← sat_eval_assertions c↣assertions,
+if c↣c↣num_quants = 0 ∧ c↣c↣num_lits = 0 then
+  add_sat_clause c↣clause_with_assertions c↣sc
+else if ¬ass_v then do
+  state_t.modify $ λst, { st with locked := ⟨c, []⟩ :: st↣locked }
+else do
+  state_t.modify $ λst, { st with passive := st↣passive↣insert c↣id c }
+
+meta def remove_passive (id : clause_id) : prover unit :=
+do state ← state_t.read, state_t.write { state with passive := state↣passive↣erase id }
+
+meta def move_locked_to_passive : prover unit := do
+locked ← flip monad.lift state_t.read (λst, st↣locked),
+new_locked ← flip filter locked (λlc, do
+  reason_vals ← mapm sat_eval_assertions lc↣reasons,
+  c_val ← sat_eval_assertions lc↣dc↣assertions,
+  if reason_vals↣for_all (λr, r = ff) ∧ c_val then do
+    state_t.modify $ λst, { st with passive := st↣passive↣insert lc↣dc↣id lc↣dc },
+    return ff
+  else
+    return tt
+),
+state_t.modify $ λst, { st with locked := new_locked }
+
+meta def move_active_to_locked : prover unit :=
+do active ← get_active, for' active↣values $ λac, do
+  c_val ← sat_eval_assertions ac↣assertions,
+  if ¬c_val then do
+     state_t.modify $ λst, { st with
+       active := st↣active↣erase ac↣id,
+       locked := ⟨ac, []⟩ :: st↣locked
+     }
+  else
+    return ()
+
+meta def move_passive_to_locked : prover unit :=
+do passive ← flip monad.lift state_t.read $ λst, st↣passive, for' passive↣to_list $ λpc, do
+  c_val ← sat_eval_assertions pc↣2↣assertions,
+  if ¬c_val then do
+    state_t.modify $ λst, { st with
+      passive := st↣passive↣erase pc↣1,
+      locked := ⟨pc↣2, []⟩ :: st↣locked
+    }
+  else
+    return ()
+
+meta def do_sat_run : prover (option expr) :=
+do sat_result ← in_sat_solver $ cdcl.run (return none),
+state_t.modify $ λst, { st with needs_sat_run := ff },
+old_model ← lift prover_state.current_model state_t.read,
+match sat_result with
+| (cdcl.result.unsat proof) := return (some proof)
+| (cdcl.result.sat new_model) := do
+    state_t.modify $ λst, { st with current_model := new_model },
+    move_locked_to_passive,
+    move_active_to_locked,
+    move_passive_to_locked,
+    return none
+end
+
+meta def take_newly_derived : prover (list derived_clause) := do
+state ← state_t.read,
+state_t.write { state with newly_derived := [] },
+return state↣newly_derived
+
+meta def remove_redundant (id : clause_id) (parents : list derived_clause) : prover unit := do
+guard $ parents↣for_all $ λp, p↣id ≠ id,
+red ← flip monad.lift state_t.read (λst, st↣active↣find id),
+match red with
+| none := return ()
+| some red := do
+let reasons := parents↣for (λp, p↣assertions),
+    assertion := red↣assertions in
+if reasons↣for_all $ λr, r↣subset_of assertion then do
+  state_t.modify $ λst, { st with active := st↣active↣erase id }
+else do
+  state_t.modify $ λst, { st with active := st↣active↣erase id,
+                                 locked := ⟨red, reasons⟩ :: st↣locked }
+end
+
+meta def inference := derived_clause → prover unit
+meta structure inf_decl := (prio : ℕ) (inf : inference)
+meta def inf_attr : user_attribute :=
+⟨ `super.inf, "inference for the super prover" ⟩
+run_command attribute.register `super.inf_attr
+
+meta def seq_inferences : list inference → inference
+| [] := λgiven, return ()
+| (inf::infs) := λgiven, do
+    inf given,
+    now_active ← get_active,
+    if rb_map.contains now_active given↣id then
+      seq_inferences infs given
+    else
+      return ()
+
+meta def simp_inference (simpl : derived_clause → prover (option clause)) : inference :=
+λgiven, do maybe_simpld ← simpl given,
+match maybe_simpld with
+| some simpld := do
+  derived_simpld ← mk_derived simpld given↣sc↣sched_now,
+  add_inferred derived_simpld,
+  remove_redundant given↣id []
+| none := return ()
+end
+
+meta def preprocessing_rule (f : list derived_clause → prover (list derived_clause)) : prover unit := do
+state ← state_t.read,
+newly_derived' ← f state↣newly_derived,
+state' ← state_t.read,
+state_t.write { state' with newly_derived := newly_derived' }
+
+meta def clause_selection_strategy := ℕ → prover clause_id
+
+namespace prover_state
+
+meta def empty (local_false : expr) : prover_state :=
+{ active := rb_map.mk _ _, passive := rb_map.mk _ _,
+  newly_derived := [], prec := [], clause_counter := 0,
+  local_false := local_false,
+  locked := [], sat_solver := cdcl.state.initial local_false,
+  current_model := rb_map.mk _ _, sat_hyps := rb_map.mk _ _, needs_sat_run := ff }
+
+meta def initial (local_false : expr) (clauses : list clause) : tactic prover_state := do
+after_setup ← for' clauses (λc,
+  let in_sos := decidable.to_bool ((contained_lconsts c↣proof)↣size = 0) in
+  do mk_derived c { priority := score.prio.immediate, in_sos := in_sos,
+                    age := 0, cost := 0 } >>= add_inferred
+) $ empty local_false,
+return after_setup.2
+
+end prover_state
+
+meta def inf_score (add_cost : ℕ) (scores : list score) : prover score := do
+age ← get_clause_count,
+return $ list.foldl score.combine { priority := score.prio.default,
+                                    in_sos := tt,
+                                    age := age,
+                                    cost := add_cost
+                                  } scores
+
+meta def inf_if_successful (add_cost : ℕ) (parent : derived_clause) (tac : tactic (list clause)) : prover unit :=
+(do inferred ← ♯tac,
+    for' inferred $ λc,
+      inf_score add_cost [parent↣sc] >>= mk_derived c >>= add_inferred)
+<|> return ()
+
+meta def simp_if_successful (parent : derived_clause) (tac : tactic (list clause)) : prover unit :=
+(do inferred ← ♯tac,
+    for' inferred $ λc,
+      mk_derived c parent↣sc↣sched_now >>= add_inferred,
+    remove_redundant parent↣id [])
+<|> return ()
+
+end super
