library/tools/super/resolution.lean
@@ -1,0 +1,57 @@
+import .clause .prover_state .utils
+open tactic monad
+
+namespace super
+
+variable gt : expr → expr → bool
+variables (ac1 ac2 : derived_clause)
+variables (c1 c2 : clause)
+variables (i1 i2 : nat)
+
+-- c1 : ... → ¬a → ...
+-- c2 : ... →  a → ...
+meta def try_resolve : tactic clause := do
+qf1 ← c1↣open_metan c1↣num_quants,
+qf2 ← c2↣open_metan c2↣num_quants,
+-- FIXME: using default transparency unifies m*n with (x*y*z)*w here ???
+unify_core transparency.reducible (qf1↣1↣get_lit i1)↣formula (qf2↣1↣get_lit i2)↣formula,
+qf1i ← qf1↣1↣inst_mvars,
+guard $ clause.is_maximal gt qf1i i1,
+op1 ← qf1↣1↣open_constn i1,
+op2 ← qf2↣1↣open_constn c2↣num_lits,
+a_in_op2 ← (op2↣2↣nth i2)↣to_monad,
+clause.meta_closure (qf1.2 ++ qf2.2) $
+  (op1↣1↣inst (op2↣1↣close_const a_in_op2)↣proof)↣close_constn (op1↣2 ++ op2↣2↣remove_nth i2)
+
+meta def try_add_resolvent : prover unit := do
+c' ← ♯ try_resolve gt ac1↣c ac2↣c i1 i2,
+inf_score 1 [ac1↣sc, ac2↣sc] >>= mk_derived c' >>= add_inferred
+
+meta def maybe_add_resolvent : prover unit :=
+try_add_resolvent gt ac1 ac2 i1 i2 <|> return ()
+
+meta def resolution_left_inf : inference :=
+take given, do active ← get_active, sequence' $ do
+  given_i ← given↣selected,
+  guard $ clause.literal.is_neg (given↣c↣get_lit given_i),
+  other ← rb_map.values active,
+  guard $ ¬given↣sc↣in_sos ∨ ¬other↣sc↣in_sos,
+  other_i ← other↣selected,
+  guard $ clause.literal.is_pos (other↣c↣get_lit other_i),
+  [maybe_add_resolvent gt other given other_i given_i]
+
+meta def resolution_right_inf : inference :=
+take given, do active ← get_active, sequence' $ do
+  given_i ← given↣selected,
+  guard $ clause.literal.is_pos (given↣c↣get_lit given_i),
+  other ← rb_map.values active,
+  guard $ ¬given↣sc↣in_sos ∨ ¬other↣sc↣in_sos,
+  other_i ← other↣selected,
+  guard $ clause.literal.is_neg (other↣c↣get_lit other_i),
+  [maybe_add_resolvent gt given other given_i other_i]
+
+@[super.inf]
+meta def resolution_inf : inf_decl := inf_decl.mk 40 $
+take given, do gt ← get_term_order, resolution_left_inf gt given >> resolution_right_inf gt given
+
+end super
