library/tools/super/selection.lean
@@ -1,0 +1,74 @@
+import .prover_state
+
+namespace super
+
+meta def simple_selection_strategy (f : (expr → expr → bool) → clause → list ℕ) : selection_strategy :=
+take dc, do gt ← get_term_order, return $
+         if dc↣selected↣empty ∧ dc↣c↣num_lits > 0
+         then { dc with selected := f gt dc↣c }
+         else dc
+
+meta def dumb_selection : selection_strategy :=
+simple_selection_strategy $ λgt c,
+match c↣lits_where clause.literal.is_neg with
+| [] := list.range c↣num_lits
+| neg_lit::_ := [neg_lit]
+end
+
+meta def selection21 : selection_strategy :=
+simple_selection_strategy $ λgt c,
+let maximal_lits := list.filter_maximal (λi j,
+  gt (c↣get_lit i)↣formula (c↣get_lit j)↣formula) (list.range c↣num_lits) in
+if list.length maximal_lits = 1 then maximal_lits else
+let neg_lits := list.filter (λi, (c↣get_lit i)↣is_neg) (list.range c↣num_lits),
+    maximal_neg_lits := list.filter_maximal (λi j,
+      gt (c↣get_lit i)↣formula (c↣get_lit j)↣formula) neg_lits in
+if ¬maximal_neg_lits^.empty then
+  list.taken 1 maximal_neg_lits
+else
+  maximal_lits
+
+meta def selection22 : selection_strategy :=
+simple_selection_strategy $ λgt c,
+let maximal_lits := list.filter_maximal (λi j,
+  gt (c↣get_lit i)↣formula (c↣get_lit j)↣formula) (list.range c↣num_lits),
+  maximal_lits_neg := list.filter (λi, (c↣get_lit i)↣is_neg) maximal_lits in
+if ¬maximal_lits_neg^.empty then
+  list.taken 1 maximal_lits_neg
+else
+  maximal_lits
+
+meta def clause_weight (c : derived_clause) : nat :=
+(c↣c↣get_lits↣for (λl, expr_size l↣formula + if l↣is_pos then 10 else 1))↣sum
+
+meta def find_minimal_by (passive : rb_map clause_id derived_clause)
+                         {A} [has_ordering A]
+                         (f : derived_clause → A) : clause_id :=
+match rb_map.min $ rb_map.of_list $ passive↣values↣for $ λc, (f c, c↣id) with
+| some id := id
+| none := nat.zero
+end
+
+meta def age_of_clause_id : name → ℕ
+| (name.mk_numeral i _) := unsigned.to_nat i
+| _ := 0
+
+meta def find_minimal_weight (passive : rb_map clause_id derived_clause) : clause_id :=
+find_minimal_by passive $ λc, (c↣sc↣priority, clause_weight c + c↣sc↣cost, c↣sc↣age, c↣id)
+
+meta def find_minimal_age (passive : rb_map clause_id derived_clause) : clause_id :=
+find_minimal_by passive $ λc, (c↣sc↣priority, c↣sc↣age, c↣id)
+
+meta def weight_clause_selection : clause_selection_strategy :=
+take iter, do state ← state_t.read, return $ find_minimal_weight state↣passive
+
+meta def oldest_clause_selection : clause_selection_strategy :=
+take iter, do state ← state_t.read, return $ find_minimal_age state↣passive
+
+meta def age_weight_clause_selection (thr mod : ℕ) : clause_selection_strategy :=
+take iter, if iter % mod < thr then
+              weight_clause_selection iter
+           else
+              oldest_clause_selection iter
+
+end super
