library/tools/super/simp.lean
@@ -1,0 +1,39 @@
+import .clause_ops .prover_state
+open tactic monad
+
+namespace super
+
+meta def prove_using_assumption : tactic unit := do
+tgt ← target,
+ass ← mk_local_def `h tgt,
+exact ass
+
+meta def simplify_capturing_assumptions (type : expr) : tactic (expr × expr × list expr) := do
+(type', heq) ← simplify default_simplify_config [] type,
+hyps ← return $ contained_lconsts type,
+hyps' ← return $ contained_lconsts_list [type', heq],
+add_hyps ← return $ list.filter (λn : expr, ¬hyps↣contains n↣local_uniq_name) hyps'↣values,
+return (type', heq, add_hyps)
+
+meta def try_simplify_left (c : clause) (i : ℕ) : tactic (list clause) :=
+on_left_at c i $ λtype, do
+  (type', heq, add_hyps) ← simplify_capturing_assumptions type,
+  hyp ← mk_local_def `h type',
+  prf  ← mk_app ``eq.mpr [heq, hyp],
+  return [(hyp::add_hyps, prf)]
+
+meta def try_simplify_right (c : clause) (i : ℕ) : tactic (list clause) :=
+on_right_at' c i $ λhyp, do
+  (type', heq, add_hyps) ← simplify_capturing_assumptions hyp↣local_type,
+  heqtype ← infer_type heq,
+  heqsymm ← mk_app ``eq.symm [heq],
+  prf  ← mk_app ``eq.mpr [heqsymm, hyp],
+  return [(add_hyps, prf)]
+
+@[super.inf]
+meta def simp_inf : inf_decl := inf_decl.mk 40 $ take given, sequence' $ do
+r ← [try_simplify_right, try_simplify_left],
+i ← list.range given↣c↣num_lits,
+[inf_if_successful 2 given (r given↣c i)]
+
+end super
