library/tools/super/subsumption.lean
@@ -1,0 +1,87 @@
+import .clause .prover_state
+open tactic monad
+
+namespace super
+
+private meta def try_subsume_core : list clause.literal → list clause.literal → tactic unit
+| [] _ := skip
+| small large := first $ do
+  i ← small↣zip_with_index, j ← large↣zip_with_index,
+  return $ do
+    unify_lit i.1 j.1,
+    try_subsume_core (small↣remove_nth i.2) (large↣remove_nth j.2)
+
+-- FIXME: this is incorrect if a quantifier is unused
+meta def try_subsume (small large : clause) : tactic unit := do
+small_open ← clause.open_metan small (clause.num_quants small),
+large_open ← clause.open_constn large (clause.num_quants large),
+guard $ small↣num_lits ≤ large↣num_lits,
+try_subsume_core small_open↣1↣get_lits large_open↣1↣get_lits
+
+meta def does_subsume (small large : clause) : tactic bool :=
+(try_subsume small large >> return tt) <|> return ff
+
+meta def does_subsume_with_assertions (small large : derived_clause) : prover bool := do
+if small↣assertions↣subset_of large↣assertions then do
+  ♯ does_subsume small↣c large↣c
+else
+  return ff
+
+meta def any_tt {m : Type → Type} [monad m] (active : rb_map clause_id derived_clause) (pred : derived_clause → m bool) : m bool :=
+active↣fold (return ff) $ λk a cont, do
+  v ← pred a, if v then return tt else cont
+
+meta def any_tt_list {m : Type → Type} [monad m] {A} (pred : A → m bool) : list A → m bool
+| [] := return ff
+| (x::xs) := do v ← pred x, if v then return tt else any_tt_list xs
+
+@[super.inf]
+meta def forward_subsumption : inf_decl := inf_decl.mk 20 $
+take given, do active ← get_active,
+sequence' $ do a ← active↣values,
+  guard $ a↣id ≠ given↣id,
+  return $ do
+    ss ← ♯ does_subsume a↣c given↣c,
+    if ss
+    then remove_redundant given↣id [a]
+    else return ()
+
+meta def forward_subsumption_pre : prover unit := preprocessing_rule $ λnew, do
+active ← get_active, filter (λn, do
+  do ss ← any_tt active (λa,
+        if a↣assertions↣subset_of n↣assertions then do
+          ♯ does_subsume a↣c n↣c
+        else
+          -- TODO: move to locked
+          return ff),
+     return (bnot ss)) new
+
+meta def subsumption_interreduction : list derived_clause → prover (list derived_clause)
+| (c::cs) := do
+  -- TODO: move to locked
+  cs_that_subsume_c ← filter (λd, does_subsume_with_assertions d c) cs,
+  if ¬cs_that_subsume_c^.empty then
+    -- TODO: update score
+    subsumption_interreduction cs
+  else do
+    cs_not_subsumed_by_c ← filter (λd, lift bnot (does_subsume_with_assertions c d)) cs,
+    cs' ← subsumption_interreduction cs_not_subsumed_by_c,
+    return (c::cs')
+| [] := return []
+
+meta def subsumption_interreduction_pre : prover unit :=
+preprocessing_rule $ λnew,
+let new' := list.sort_on (λc : derived_clause, c↣c↣num_lits) new in
+subsumption_interreduction new'
+
+meta def keys_where_tt {m} {K V : Type} [monad m] (active : rb_map K V) (pred : V → m bool) : m (list K) :=
+@rb_map.fold _ _ (m (list K)) active (return []) $ λk a cont, do
+  v ← pred a, rest ← cont, return $ if v then k::rest else rest
+
+@[super.inf]
+meta def backward_subsumption : inf_decl := inf_decl.mk 20 $ λgiven, do
+active ← get_active,
+ss ← ♯ keys_where_tt active (λa, does_subsume given↣c a↣c),
+sequence' $ do id ← ss, guard (id ≠ given↣id), [remove_redundant id [given]]
+
+end super
