library/tools/super/superposition.lean
@@ -1,0 +1,137 @@
+import .clause .prover_state .utils
+open tactic monad expr
+
+namespace super
+
+meta def get_rwr_positions : expr → list (list ℕ)
+| (app a b) := [[]] ++
+  do arg ← list.zip_with_index (get_app_args (app a b)),
+     pos ← get_rwr_positions arg↣1,
+     [arg↣2 :: pos]
+| (var _) := []
+| e := [[]]
+
+meta def get_position : expr → list ℕ → expr
+| (app a b) (p::ps) :=
+match list.nth (get_app_args (app a b)) p with
+| some arg := get_position arg ps
+| none := (app a b)
+end
+| e _ := e
+
+meta def replace_position (v : expr) : expr → list ℕ → expr
+| (app a b) (p::ps) :=
+let args := get_app_args (app a b) in
+match args↣nth p with
+| some arg := app_of_list a↣get_app_fn $ args↣update_nth p $ replace_position arg ps
+| none := app a b
+end
+| e [] := v
+| e _ := e
+
+variable gt : expr → expr → bool
+variables (c1 c2 : clause)
+variables (ac1 ac2 : derived_clause)
+variables (i1 i2 : nat)
+variable pos : list ℕ
+variable ltr : bool
+variable congr_ax : name
+
+lemma {u v w} sup_ltr (F : Type u) (A : Type v) (a1 a2) (f : A → Type w) : (f a1 → F) → f a2 → a1 = a2 → F :=
+take hnfa1 hfa2 heq, hnfa1 (@eq.rec A a2 f hfa2 a1 heq↣symm)
+lemma {u v w} sup_rtl (F : Type u) (A : Type v) (a1 a2) (f : A → Type w) : (f a1 → F) → f a2 → a2 = a1 → F :=
+take hnfa1 hfa2 heq, hnfa1 (@eq.rec A a2 f hfa2 a1 heq)
+
+meta def is_eq_dir (e : expr) (ltr : bool) : option (expr × expr) :=
+match is_eq e with
+| some (lhs, rhs) := if ltr then some (lhs, rhs) else some (rhs, lhs)
+| none := none
+end
+
+meta def try_sup : tactic clause := do
+guard $ (c1↣get_lit i1)↣is_pos,
+qf1 ← c1↣open_metan c1↣num_quants,
+qf2 ← c2↣open_metan c2↣num_quants,
+(rwr_from, rwr_to) ← (is_eq_dir (qf1↣1↣get_lit i1)↣formula ltr)↣to_monad,
+atom ← return (qf2↣1↣get_lit i2)↣formula,
+eq_type ← infer_type rwr_from,
+atom_at_pos_type ← infer_type $ get_position atom pos,
+unify eq_type atom_at_pos_type,
+unify_core transparency.none rwr_from (get_position atom pos),
+rwr_from' ← instantiate_mvars rwr_from,
+rwr_to' ← instantiate_mvars rwr_to,
+guard $ ¬gt rwr_to' rwr_from',
+rwr_ctx_varn ← mk_fresh_name,
+abs_rwr_ctx ← return $
+  lam rwr_ctx_varn binder_info.default eq_type
+  (if (qf2↣1↣get_lit i2)↣is_neg
+   then replace_position (mk_var 0) atom pos
+   else imp (replace_position (mk_var 0) atom pos) c2↣local_false),
+lf_univ ← infer_univ c1↣local_false,
+univ ← infer_univ eq_type,
+atom_univ ← infer_univ atom,
+op1 ← qf1↣1↣open_constn i1,
+op2 ← qf2↣1↣open_constn c2↣num_lits,
+hi2 ← (op2↣2↣nth i2)↣to_monad,
+new_atom ← whnf $ app abs_rwr_ctx rwr_to',
+new_hi2 ← return $ local_const hi2↣local_uniq_name `H binder_info.default new_atom,
+new_fin_prf ←
+  return $ app_of_list (const congr_ax [lf_univ, univ, atom_univ]) [c1↣local_false, eq_type, rwr_from, rwr_to,
+            abs_rwr_ctx, (op2↣1↣close_const hi2)↣proof, new_hi2],
+clause.meta_closure (qf1↣2 ++ qf2↣2) $ (op1↣1↣inst new_fin_prf)↣close_constn (op1↣2 ++ op2↣2↣update_nth i2 new_hi2)
+
+example (i : Type) (a b : i) (p : i → Prop) (H : a = b) (Hpa : p a) : true := by do
+H ← get_local `H >>= clause.of_classical_proof,
+Hpa ← get_local `Hpa >>= clause.of_classical_proof,
+a ← get_local `a,
+try_sup (λx y, ff) H Hpa 0 0 [0] tt ``super.sup_ltr >>= clause.validate,
+to_expr `(trivial) >>= apply
+
+example (i : Type) (a b : i) (p : i → Prop) (H : a = b) (Hpa : p a → false) (Hpb : p b → false) : true := by do
+H ← get_local `H >>= clause.of_classical_proof,
+Hpa ← get_local `Hpa >>= clause.of_classical_proof,
+Hpb ← get_local `Hpb >>= clause.of_classical_proof,
+try_sup (λx y, ff) H Hpa 0 0 [0] tt ``super.sup_ltr >>= clause.validate,
+try_sup (λx y, ff) H Hpb 0 0 [0] ff ``super.sup_rtl >>= clause.validate,
+to_expr `(trivial) >>= apply
+
+meta def rwr_positions (c : clause) (i : nat) : list (list ℕ) :=
+get_rwr_positions (c↣get_lit i)↣formula
+
+meta def try_add_sup : prover unit :=
+(do c' ← ♯ try_sup gt ac1↣c ac2↣c i1 i2 pos ltr congr_ax,
+    inf_score 2 [ac1↣sc, ac2↣sc] >>= mk_derived c' >>= add_inferred)
+  <|> return ()
+
+meta def superposition_back_inf : inference :=
+take given, do active ← get_active, sequence' $ do
+  given_i ← given↣selected,
+  guard (given↣c↣get_lit given_i)↣is_pos,
+  option.to_monad $ is_eq (given↣c↣get_lit given_i)↣formula,
+  other ← rb_map.values active,
+  guard $ ¬given↣sc↣in_sos ∨ ¬other↣sc↣in_sos,
+  other_i ← other↣selected,
+  pos ← rwr_positions other↣c other_i,
+  -- FIXME(gabriel): ``sup_ltr fails to resolve at runtime
+  [do try_add_sup gt given other given_i other_i pos tt ``super.sup_ltr,
+      try_add_sup gt given other given_i other_i pos ff ``super.sup_rtl]
+
+meta def superposition_fwd_inf : inference :=
+take given, do active ← get_active, sequence' $ do
+  given_i ← given↣selected,
+  other ← rb_map.values active,
+  guard $ ¬given↣sc↣in_sos ∨ ¬other↣sc↣in_sos,
+  other_i ← other↣selected,
+  guard (other↣c↣get_lit other_i)↣is_pos,
+  option.to_monad $ is_eq (other↣c↣get_lit other_i)↣formula,
+  pos ← rwr_positions given↣c given_i,
+  [do try_add_sup gt other given other_i given_i pos tt ``super.sup_ltr,
+      try_add_sup gt other given other_i given_i pos ff ``super.sup_rtl]
+
+@[super.inf]
+meta def superposition_inf : inf_decl := inf_decl.mk 40 $
+take given, do gt ← get_term_order,
+superposition_fwd_inf gt given,
+superposition_back_inf gt given
+
+end super
