library/tools/super/trim.lean
@@ -1,0 +1,63 @@
+import .utils
+open monad expr tactic
+
+namespace super
+
+meta def count_var_occs : unsigned → expr → ℕ
+| k (var k')              := if k = k' then 1 else 0
+| _ (sort _)              := 0
+| _ (const _ _)           := 0
+| _ (mvar _ _)            := 0
+| k (local_const _ _ _ t) := count_var_occs k t
+| k (app a b)             := count_var_occs k a + count_var_occs k b
+| k (lam _ _ t b)         := count_var_occs k t + count_var_occs k^.succ b
+| k (pi _ _ t b)          := count_var_occs k t + count_var_occs k^.succ b
+| k (elet _ t v b)        := count_var_occs k t + count_var_occs k v + count_var_occs k^.succ b
+| _ (macro _ _ _)         := 0 -- TODO(gabriel)
+
+-- TODO(gabriel): rewrite using conversions
+meta def trim : expr → tactic expr
+| (app (lam n m d b) arg) :=
+  if has_var b = ff ∨ count_var_occs 0 b ≤ 1 then
+    trim (instantiate_var b arg)
+  else
+    lift₂ app (trim (lam n m d b)) (trim arg)
+| (app a b) := lift₂ app (trim a) (trim b)
+| (lam n m d b) := do
+  x ← mk_local' `x m d,
+  b' ← trim (instantiate_var b x),
+  return $ lam n m d (abstract_local b' x^.local_uniq_name)
+| (elet n t v b) :=
+  if has_var b then do
+    x ← mk_local_def `x t,
+    b' ← trim (instantiate_var b x),
+    return $ elet n t v (abstract_local b' x^.local_uniq_name)
+  else
+    trim b
+| e := return e
+
+-- iterate trim until convergence
+meta def trim' : expr → tactic expr
+| e := do e' ← trim e,
+          if e =ₐ e' then
+            return e
+          else
+            trim' e'
+
+open tactic
+
+meta def with_trim {α} (tac : tactic α) : tactic α := do
+gs ← get_goals,
+match gs with
+| (g::gs) := do
+  g' ← infer_type g >>= mk_meta_var,
+  set_goals [g'],
+  r ← tac,
+  now,
+  set_goals (g::gs),
+  instantiate_mvars g' >>= trim' >>= exact,
+  return r
+| [] := fail "no goal"
+end
+
+end super
