library/tools/super/utils.lean
@@ -1,0 +1,149 @@
+open tactic expr list
+
+meta def get_metas : expr → list expr
+| (var _) := []
+| (sort _) := []
+| (const _ _) := []
+| (mvar n t) := expr.mvar n t :: get_metas t
+| (local_const _ _ _ t) := get_metas t
+| (app a b) := get_metas a ++ get_metas b
+| (lam _ _ d b) := get_metas d ++ get_metas b
+| (pi _ _ d b) := get_metas d ++ get_metas b
+| (elet _ t v b) := get_metas t ++ get_metas v ++ get_metas b
+| (macro _ _ _) := []
+
+meta def get_meta_type : expr → expr
+| (mvar _ t) := t
+| _ := mk_var 0
+
+-- TODO(gabriel): think about how to handle the avalanche of implicit arguments
+meta def expr_size : expr → nat
+| (var _) := 1
+| (sort _) := 1
+| (const _ _) := 1
+| (mvar n t) := 1
+| (local_const _ _ _ _) := 1
+| (app a b) := expr_size a + expr_size b
+| (lam _ _ d b) := 1 + expr_size b
+| (pi _ _ d b) := 1 + expr_size b
+| (elet _ t v b) := 1 + expr_size v + expr_size b
+| (macro _ _ _) := 1
+
+namespace ordering
+
+def is_lt {A} [has_ordering A] (x y : A) : bool :=
+match has_ordering.cmp x y with ordering.lt := tt | _ := ff end
+
+end ordering
+
+namespace list
+
+meta def nub {A} [has_ordering A] (l : list A) : list A :=
+rb_map.keys (rb_map.set_of_list l)
+
+meta def nub_on {A B} [has_ordering B] (f : A → B) (l : list A) : list A :=
+rb_map.values (rb_map.of_list (map (λx, (f x, x)) l))
+
+def nub_on' {A B} [decidable_eq B] (f : A → B) : list A → list A
+| [] := []
+| (x::xs) := x :: filter (λy, f x ≠ f y) (nub_on' xs)
+
+def for_all {A} (l : list A) (p : A → Prop) [decidable_pred p] : bool :=
+list.all l (λx, to_bool (p x))
+
+def exists_ {A} (l : list A) (p : A → Prop) [decidable_pred p] : bool :=
+list.any l (λx, to_bool (p x))
+
+def subset_of {A} [decidable_eq A] (xs ys : list A) :=
+xs↣for_all (λx, x ∈ ys)
+
+def filter_maximal {A} (gt : A → A → bool) (l : list A) : list A :=
+filter (λx, l↣for_all (λy, ¬gt y x)) l
+
+private def zip_with_index' {A} : ℕ → list A → list (A × ℕ)
+| _ nil := nil
+| i (x::xs) := (x,i) :: zip_with_index' (i+1) xs
+
+def zip_with_index {A} : list A → list (A × ℕ) :=
+zip_with_index' 0
+
+def partition {A} (pred : A → Prop) [decidable_pred pred] : list A → list A × list A
+| (x::xs) := match partition xs with (ts,fs) := if pred x then (x::ts, fs) else (ts, x::fs) end
+| [] := ([],[])
+
+meta def merge_sorted {A} [has_ordering A] : list A → list A → list A
+| [] ys := ys
+| xs [] := xs
+| (x::xs) (y::ys) :=
+  if ordering.is_lt x y then
+    x :: merge_sorted xs (y::ys)
+  else
+    y :: merge_sorted (x::xs) ys
+
+meta def sort {A} [has_ordering A] : list A → list A
+| (x::xs) :=
+  let (smaller, greater_eq) := partition (λy, ordering.is_lt y x) xs in
+  merge_sorted (sort smaller) (x :: sort greater_eq)
+| [] := []
+
+meta def sort_on {A B} (f : A → B) [has_ordering B] : list A → list A :=
+@sort _ ⟨λx y, has_ordering.cmp (f x) (f y)⟩
+
+end list
+
+meta def name_of_funsym : expr → name
+| (local_const uniq _ _ _) := uniq
+| (const n _) := n
+| _ := name.anonymous
+
+private meta def contained_funsyms' : expr → rb_map name expr → rb_map name expr
+| (var _) m := m
+| (sort _) m := m
+| (const n ls) m := rb_map.insert m n (const n ls)
+| (mvar _ t) m := contained_funsyms' t m
+| (local_const uniq pp bi t) m := rb_map.insert m uniq (local_const uniq pp bi t)
+| (app a b) m := contained_funsyms' a (contained_funsyms' b m)
+| (lam _ _ d b) m := contained_funsyms' d (contained_funsyms' b m)
+| (pi _ _ d b) m := contained_funsyms' d (contained_funsyms' b m)
+| (elet _ t v b) m := contained_funsyms' t (contained_funsyms' v (contained_funsyms' b m))
+| (macro _ _ _) m := m
+
+meta def contained_funsyms (e : expr) : rb_map name expr :=
+contained_funsyms' e (rb_map.mk name expr)
+
+private meta def contained_lconsts' : expr → rb_map name expr → rb_map name expr
+| (var _) m := m
+| (sort _) m := m
+| (const _ _) m := m
+| (mvar _ t) m := contained_lconsts' t m
+| (local_const uniq pp bi t) m := contained_lconsts' t (rb_map.insert m uniq (local_const uniq pp bi t))
+| (app a b) m := contained_lconsts' a (contained_lconsts' b m)
+| (lam _ _ d b) m := contained_lconsts' d (contained_lconsts' b m)
+| (pi _ _ d b) m := contained_lconsts' d (contained_lconsts' b m)
+| (elet _ t v b) m := contained_lconsts' t (contained_lconsts' v (contained_lconsts' b m))
+| (macro _ _ _) m := m
+
+meta def contained_lconsts (e : expr) : rb_map name expr :=
+contained_lconsts' e (rb_map.mk name expr)
+
+meta def contained_lconsts_list (es : list expr) : rb_map name expr :=
+list.foldl (λlcs e, contained_lconsts' e lcs) (rb_map.mk name expr) es
+
+namespace tactic
+
+meta def infer_univ (type : expr) : tactic level :=
+do sort_of_type ← infer_type type >>= whnf,
+match sort_of_type with
+| sort lvl := return lvl
+| not_sort := do fmt ← pp not_sort,
+                 fail $ to_fmt "cannot get universe level of sort: " ++ fmt
+end
+
+end tactic
+
+namespace nat
+
+def min (m n : ℕ) := if m < n then m else n
+def max (m n : ℕ) := if m > n then m else n
+
+end nat
